this is going no where and imo its pointless

Translation/Term.lean
@@ -4,7 +4,11 @@ import Surface.Ty
 import Surface.Term
 
 import Translation.Ty
+import Surface.BiTyping
+
 open LeanSubst
+
+
 
 @[simp, grind]
 def Surface.Term.translate (G : Core.GlobalEnv) (Δ : Core.KindEnv) (Γ : Core.TyEnv) :
@@ -50,35 +54,31 @@ def Surface.Term.type_directed_translate (G : Core.GlobalEnv) (Δ : Core.KindEnv
   let t' <- t.type_directed_translate G Δ (A.translate :: Γ) B'
   if A' == A.translate
   then return λ[A.translate] t' else none
--- Elimination forms are a little annoying
-| .match (n := n) s ps cs d => do -- also maybe store the type of the scrutinee to eliminate
-  let s' <- s.translate G Δ Γ
-  let ops' : Vect n (Option Core.Term) := (λ i => (ps i).translate G Δ Γ)
-  let ps' <- ops'.seq
-  let ocs' : Vect n (Option Core.Term) := (λ i => (cs i).translate G Δ Γ)
-  let cs' <- ocs'.seq
-  let d' <- d.type_directed_translate G Δ Γ τ
-  return match! n s' ps' cs' d'
-| t => do
-  let (x, sp) <- t.spine
-  let hτ <- Core.lookup_type G x
-  let (t', r) <- List.foldlM (λ (acct, τ) x =>
-               match argh : τ, x with
-               | .all K τ, .type A =>
-                 -- K better be kind of A, but we can't do that yet.
-                 let A' := A.translate
-                 let σ : Subst Core.Ty := (su A')::+0
-                 return (acct •[ A' ], τ[σ])
-               | .arrow A B, .term t => do
-                 let t' <- t.type_directed_translate G Δ Γ A
-                 return (acct • t', B)
-               | _ , _ => none)
-               (g#x, hτ) sp
-  if r == τ then return t' else none
-termination_by t => t.size
-decreasing_by (
-all_goals try (simp at *)
-· omega
-· sorry
+| _ => none
 
-)
+
+def Surface.Term.check_type_translate (G : Core.GlobalEnv) (Δ : Core.KindEnv) (Γ : Core.TyEnv) :
+  Surface.Term -> Option Core.Term
+| .match (n := n) s ps cs d => do
+  let s' <- s.check_type_translate G Δ Γ
+  let ops' : Vect n (Option Core.Term) := (λ i => (ps i).check_type_translate G Δ Γ)
+  let ps' <- ops'.seq
+  let ocs' : Vect n (Option Core.Term) := (λ i => (cs i).check_type_translate G Δ Γ)
+  let cs' <- ocs'.seq
+  let d' <- d.check_type_translate G Δ Γ
+  return match! n s' ps' cs' d'
+| .app t1 t2 => do
+  let t1' <- t1.check_type_translate G Δ Γ
+  let t2' <- t2.check_type_translate G Δ Γ
+  return (t1' • t2')
+| .appt t1 t2 => do
+  let t1' <- t1.check_type_translate G Δ Γ
+  let t2' <- t2.translate
+  return (t1' •[ t2' ])
+| _ => none
+
+
+def Surface.Term.check_infer_translate (G : Core.GlobalEnv) (Δ : Core.KindEnv) (Γ : Core.TyEnv) :
+  Mode -> Surface.Term -> Option Core.Term
+| chk => Surface.Term.type_directed_translate G Δ Γ T.translate
+| inf => Surface.Term.check_type_translate G Δ Γ
