Surface/BiTyping.lean
@@ -1,0 +1,67 @@
+import Surface.Term
+import Surface.Ty
+
+import Surface.Typing
+
+namespace Surface
+
+inductive Mode : Type where
+| chk | syn
+
+@[simp]
+abbrev BiTypingArgs : Mode -> Type
+| .chk => Term × Ty
+| .syn => Term
+
+inductive BiTyping (G : GlobalEnv) :  KindEnv -> TyEnv -> (m : Mode) -> (BiTypingArgs m) -> Prop where
+| var :
+  Γ[x]? = some A ->
+  G&Δ ⊢s A : .base b ->
+  BiTyping G Δ Γ .syn (`#x)
+-- | global :
+--   lookup_type G x = some A ->
+--   G&Δ ⊢s A : .base b ->
+--   BiTyping G Δ Γ .syn g`#x
+
+-- | mtch (CTy : Vect n Ty)
+--        (PTy : Vect n Ty)
+--        (pats : Vect n Term)
+--        (cs : Vect n Term) :
+--   BiTyping G Δ Γ syn s ->
+--   ValidTyHeadVariable R (is_data G) ->
+--   BiTyping G chk Δ Γ c T -> -- catch all term is of type T
+--   (∀ i, ValidHeadVariable (pats i) (is_ctor G)) -> -- patterns are of the right shape
+--   (∀ i, BiTyping G chk Δ Γ (pats i) (PTy i)) -> -- each pattern has a type
+--   (∀ i, StableTypeMatch Δ (PTy i) R) -> -- the pattern type has a return type that matches datatype
+--   (∀ i, BiTyping G chk Δ Γ (cs i) (CTy i)) -> -- each case match has a type
+--   (∀ i, PrefixTypeMatch Δ (PTy i) (CTy i) T) -> -- patten type and case type
+--   BiTyping G Δ Γ chk ((matchˢ! s pats cs c),  T)
+
+-- | appt :
+--   BiTyping G syn Δ Γ f (`∀[K] P) ->
+--   G&Δ ⊢s a : K ->
+--   P' = P[.su a :: +0:Ty] ->
+--   BiTyping G chk Δ Γ (f `•[a]) P'
+
+-- | app :
+--   G&Δ ⊢s A : `★ ->
+--   BiTyping G Δ Γ .syn f ->
+--   BiTyping G Δ Γ .chk (a , A) ->
+--   BiTyping G Δ Γ chk (f `• a , B)
+
+-- --------------------------------------------------------------------------------------
+-- ---- Terms
+-- --------------------------------------------------------------------------------------
+-- | lam :
+--   G&Δ ⊢s A : .base b1 ->
+--   BiTyping G inf Δ (A::Γ) t B ->
+--   BiTyping G inf Δ Γ (λˢ[A] t) (A `-:> B)
+-- | lamt :
+--   Kinding G Δ (`∀[K]P) `★ ->
+--   BiTyping G inf (K::Δ) (Γ.map (·[+1])) t P ->
+--   BiTyping G inf Δ Γ (Λˢ[K] t) (`∀[K] P)
+
+notation:170 G:170 "&" Δ:170 "," Γ:170 " ⊢s " t:170 " => " => BiTyping G Mode.syn Δ Γ t
+notation:170 G:170 "&" Δ:170 "," Γ:170 " ⊢s " t:170 " <= " A:170 => BiTyping G Mode.chk Δ Γ t A
+
+end Surface
