Translation/Term/Lemmas2D.lean
@@ -1,0 +1,67 @@
+import Core.Ty
+import Core.Term
+import Core.Metatheory.Determined.Definition
+import Surface.Ty
+import Surface.Term
+
+import Translation.Ty
+import Translation.Term
+
+import Translation.Ty.Lemmas
+
+import Translation.Ty
+import Translation.Term
+import Translation.Global
+import Core.Typing
+import Surface.BiTyping
+import Core.Metatheory.Inversion
+import Core.Term.Spine
+import Surface.Typing
+import Surface.Metatheory.Inversion
+import Translation.Rename
+
+open LeanSubst
+
+namespace Surface
+
+theorem Translation.Term.Sound_2d_syn (G : Surface.GlobalEnv) :
+  ⊢s G ->
+  G&Δ,Γ ⊢s t => T ->
+
+
+  G.translate = G' ->
+  ⊢ G' ->
+
+  Δ.translate = Δ' ->
+  Γ.translate = Γ' ->
+
+
+  ∃ t', t.check_type_translate G' Δ' Γ' = some t' ∧
+        t'.Determined ∧
+        G'&Δ',Γ' ⊢ t' : T.translate := by sorry
+
+
+
+theorem Translation.Term.Sound_2d_chk (G : Surface.GlobalEnv) :
+  ⊢s G ->
+  G&Δ,Γ ⊢s t <= T ->
+
+
+  G.translate = G' ->
+  ⊢ G' ->
+
+  Δ.translate = Δ' ->
+  Γ.translate = Γ' ->
+
+
+  ∃ t', t.type_directed_translate G' Δ' Γ' T.translate = some t' ∧
+        t'.Determined ∧
+        G'&Δ',Γ' ⊢ t' : T.translate := by
+intro wf j h1 h2 h3 h4
+
+sorry
+
+
+
+
+end Surface
